rocq-osiris/theories/program_logic/rules/auxiliary_rules.v
@@ -159,7 +159,7 @@ Section imp_eval.
 
   Lemma imp_sitems_extend sitems x Q η δ :
     (∀ l, l ↦ #() -∗
-          imp eval_sitems ((x, VLoc l) :: η, (x, VLoc l) :: δ) sitems @ E <| Ψ |> ⟨⟨ ζ ⟩⟩ {{ Q }}) -∗
+          imp eval_sitems ((x, #l) :: η, (x, #l) :: δ) sitems @ E <| Ψ |> ⟨⟨ ζ ⟩⟩ {{ Q }}) -∗
     imp eval_sitems (η,δ) ((IExtend [x]) :: sitems) @ E <| Ψ |> ⟨⟨ ζ ⟩⟩ {{ Q }}.
   Proof.
     iIntros "Hcov".
@@ -169,7 +169,7 @@ Section imp_eval.
       iIntros (l) "Hl"; simpl; iApply imp_ret. reflexivity.
       Unshelve.
       2: (apply (λ ηδ,
-                   (∃ l, ⌜ηδ = ((x, VLoc l) :: η, (x, VLoc l):: δ)⌝ ∗ l ↦ VUnit)%I)).
+                   (∃ l, ⌜ηδ = ((x, #l) :: η, (x, #l):: δ)⌝ ∗ l ↦ VUnit)%I)).
       simpl.
       iExists l; iFrame. iPureIntro; reflexivity. }
     iIntros ([??]) "(% & -> & Hl)".
@@ -218,7 +218,7 @@ Section imp_eval.
 
   Lemma imp_type_extension_cons e es Q :
     ▷ (∀ l, l ↦ #() -∗
-            imp eval_type_extensions es @ E <| Ψ |> ⟨⟨ ζ ⟩⟩ {{ λ δ, Q ((e, VLoc l) :: δ) }}) -∗
+            imp eval_type_extensions es @ E <| Ψ |> ⟨⟨ ζ ⟩⟩ {{ λ δ, Q ((e, #l) :: δ) }}) -∗
     imp eval_type_extensions (e :: es) @ E <| Ψ |> ⟨⟨ ζ ⟩⟩ {{ Q }}.
   Proof.
     iIntros "Hes". simpl.
